$\angle{PSQ}$ is the angle between $\vec{SP}$ and $\vec{SQ}$

$\angle{PSR}$ is the angle between $\vec{SP}$ and $\vec{SR}$
\\
Finding the Scalar Products:
$$(\vec{P} - \vec{S})^T(\vec{Q} - \vec{S}) = \norm{\vec{P} - \vec{S}}\norm{\vec{Q} - \vec{S}}\cos{\angle{PSQ}}$$
$$(\myvec{2.25\\3.3072} - \myvec{\frac{8}{3}\\0})^T(\myvec{0\\0} - \myvec{\frac{8}{3}\\0}) = (3.33)\frac{8}{3}\cos{\angle{PSQ}}$$
$$\cos{\angle{PSQ}} = \frac{\myvec{-0.416\\3.3072}.\myvec{\frac{-8}{3}\\0}}{(3.33).\frac{8}{3}}$$
$$\cos{\angle{PSQ}} = 0.1249$$
$$\angle{PSQ} = \cos^{-1}{0.1249} = 82.82\degree$$

$$(\vec{P} - \vec{S})^T(\vec{R} - \vec{S}) = \norm{\vec{P} - \vec{S}}\norm{\vec{R} - \vec{S}}\cos{\angle{PSR}}$$
$$(\myvec{2.25\\3.3072} - \myvec{\frac{8}{3}\\0})^T(\myvec{6\\0} - \myvec{\frac{8}{3}\\0}) = (3.33)\frac{10}{3}\cos{\angle{PSR}}$$
$$\cos{\angle{PSR}} = \frac{\myvec{-0.416\\3.3072}.\myvec{3.33\\0}}{(3.33).\frac{10}{3}}$$
$$\cos{\angle{PSR}} = -0.1248$$
$$\angle{PSR} = \cos^{-1}{-0.1248} = 97.17\degree$$

Therefore, $\angle{PSR} > \angle{PSQ}$
